Modified map implementation

elo-coq/Map.v
@@ -2,36 +2,25 @@ From Coq Require Import Strings.String.
 From Coq Require Import Lists.List.
 From Elo Require Export Array.
 
-(* Inductive list2 {A B: Type} : Type :=
-  | nil2
-  | cons2 (a : A) (b : B) (m : list2).
+Local Definition map' (A : Type) := string -> A. (* total map *)
 
-Definition map A := @list2 string A.
+Local Definition empty' {A : Type} v : map' A := (fun _ => v).
 
-Local Fixpoint index_of' {A} (m : map A) (k : string) (i : nat) :=
-  match m with
-  | nil2 => None
-  | cons2 k' v' m' => if eqb k k'
-    then Some (i, v')
-    else index_of' m' k (i + 1)
-  end.
+Local Definition update' {A : Type} (m : map' A) k v :=
+  fun k' => if String.eqb k k' then v else m k'.
 
-Definition index_of {A} m k := @index_of' A m k 0.
+Definition map (A : Type) := map' (option A). (* partial map *)
 
-Definition update {A} (m : map A) k v :=
-  match index_of m k with
-  | None => m ++ (cons2 k v nil2)
-  | Some (i, _) => nil2
-  end.
+Definition empty {A : Type} : map A := empty' None.
 
-Definition lookup {A} (m : map A) k :=
-  match index_of m k with
-  | None => None
-  | Some (_, v) => Some v
-  end.
-*)
+Definition update {A : Type} (m : map A) k v :=
+  update' m k (Some v).
 
-Definition map A := list (string * A).
+Definition lookup {A : Type} (m : map A) k := m k.
+
+
+
+(* Definition map A := list (string * A).
 
 Local Fixpoint index_of' {A} (m : map A) (k : string) (i : nat) :=
   match m with
@@ -53,4 +42,4 @@ Definition lookup {A} (m : map A) k :=
   match index_of m k with
   | None => None
   | Some (_, v) => Some v
-  end.
+  end. *)
